coq/lib/Semantics/Properties.v
@@ -1,0 +1,132 @@
+Require Export CoqRecon.Semantics.DeclTyping CoqRecon.Semantics.Reduce.
+
+Section Canon.
+  Variable v : term.
+
+  Hypothesis Hv : value v.
+  
+  Lemma canon_abs : forall t t',
+      ∅ ⊨ v ∴ t → t' -> exists x e, v = λ x ⇒ e.
+  Proof.
+    intros t t' Ht; inv Hv; inv Ht; eauto.
+  Qed.
+
+  Lemma canon_nat : ∅ ⊨ v ∴ TNat -> exists n : nat, v = n.
+  Proof.
+    intros Ht; inv Hv; inv Ht; eauto.
+  Qed.
+
+  Lemma canon_bool : ∅ ⊨ v ∴ TBool -> exists b : bool, v = b.
+  Proof.
+    intros Ht; inv Hv; inv Ht; eauto.
+  Qed.
+End Canon.
+
+Section Progress.
+  Local Hint Constructors value : core.
+  Local Hint Constructors typing : core.
+
+  Local Hint Extern 0 =>
+  match goal with
+  | |- context [if ?b then _ else _] =>
+    destruct b eqn:?; simpl
+  end : core.
+
+  Theorem prog : forall e t,
+      ∅ ⊨ e ∴ t -> value e \/ exists e', rd e = Some e'.
+  Proof.
+    intro e;
+      induction e as
+        [ x
+        | x e IHe
+        | e1 IHe1 e2 IHe2
+        | n | b
+        | e1 IHe1 e2 IHe2 e3 IHe3
+        | o e1 IHe1 e2 IHe2
+        | x e1 IHe1 e2 IHe2 ];
+      intros t Ht; inv Ht; simpl;
+        repeat match goal with
+               | H: op_typs _ _ _ |- _ => inv H
+               | IH: (forall t, ?g ⊨ ?e ∴ t -> _), H : ?g ⊨ ?e ∴ ?t
+                 |- _ => pose proof IH t H as [? | [? ?]]; clear IH
+               | H: ∅ ⊨ ?v ∴ _ → _, Hv: value ?v
+                 |- _ => pose proof canon_abs v Hv _ _ H as (? & ? & ?);
+                         clear Hv; subst; simpl
+               | H: ∅ ⊨ ?v ∴ TNat, Hv: value ?v
+                 |- _ => pose proof canon_nat v Hv H as (? & ?);
+                         clear Hv; subst; simpl
+               | H: ∅ ⊨ ?v ∴ TBool, Hv: value ?v
+                 |- _ => pose proof canon_bool v Hv H as (? & ?);
+                         clear Hv; subst; simpl
+               | H: rd ?e = Some _ |- context [rd ?e] => rewrite H; clear H
+               | H: bound _ _ ∅ |- _ => unfold bound, "∅" in H; discriminate
+               end;
+        maybe_simpl; eauto;
+          try (destruct e1; eauto; assumption);
+          try (destruct e2; eauto; assumption);
+          try (destruct e1; destruct e2; eauto; assumption);
+          try (destruct e1; eauto;
+               match goal with
+               | H: _ ⊨ Nat _ ∴ TBool |- _ => inv H
+               | H: _ ⊨ Bool _ ∴ TNat |- _ => inv H
+               end; contradiction).
+  Qed.
+End Progress.
+
+Section Sub.
+  Local Hint Constructors typing : core.
+  Hint Rewrite (@bind_same string typ) : core.
+
+  Lemma weakening : forall g e t,
+      g ⊨ e ∴ t -> forall g', incl g g' -> g' ⊨ e ∴ t.
+  Proof.
+    unfold incl, bound;
+      intros g e t Hget; induction Hget;
+        intros g' HI; unfold bound in *;
+          simpl in *; eauto.
+    - constructor. firstorder.
+    - constructor.
+      apply IHHget; intuition.
+      unfold bind in *; repeat dispatch_eqdec; auto.
+    - econstructor; eauto.
+      apply IHHget2; intuition.
+      unfold bind in *; repeat dispatch_eqdec; auto.
+  Qed.
+  
+  Lemma empty_ctx : forall e t,
+      ∅ ⊨ e ∴ t -> forall g, g ⊨ e ∴ t.
+  Proof.
+    intros e t H g.
+    apply weakening with (g' := g) in H; auto.
+    unfold incl, bound, "∅". discriminate.
+  Qed.
+
+  Local Hint Resolve empty_ctx : core.
+  
+  Lemma sub_lemma : forall e e' t t' x g,
+      (x ↦ t';; g) ⊨ e ∴ t -> ∅ ⊨ e' ∴ t' -> g ⊨ ⟦x:=e'⟧ e ∴ t.
+  Proof.
+    intro e;
+      induction e as
+        [ x
+        | x e IHe
+        | e1 IHe1 e2 IHe2
+        | n | b
+        | e1 IHe1 e2 IHe2 e3 IHe3
+        | o e1 IHe1 e2 IHe2
+        | x e1 IHe1 e2 IHe2 ];
+      intros e' t t' y g He He'; inv He; simpl;
+        unfold bound in *; eauto.
+    - dispatch_eqdec.
+      + rewrite bind_sound in H0; inv H0; auto.
+      + rewrite bind_complete in H0; auto.
+    - dispatch_eqdec; autorewrite with core in *; eauto.
+      rewrite bind_diff_comm in H2 by auto; eauto.
+    - dispatch_eqdec; autorewrite with core in *; eauto.
+      rewrite bind_diff_comm in H4 by auto; eauto.
+  Qed.
+End Sub.
+
+Section Preservation.
+  (* TODO *)
+End Preservation.
