coq/lib/Semantics/Reduce.v
@@ -1,0 +1,49 @@
+Require Export CoqRecon.Syntax.Term CoqRecon.Util.EqDecInst.
+
+Reserved Notation "'⟦' x ':=' v '⟧' e"
+         (at level 20, right associativity).
+
+Open Scope term_scope.
+
+(** Capture-avoiding Substitution. *)
+Fixpoint sub (x : string) (v e : term) : term :=
+  match e with
+  | Var y   => if equiv_dec x y then v else y
+  | λ y ⇒ e => if equiv_dec x y then λ y ⇒ e else λ y ⇒ ⟦x:=v⟧ e
+  | e1 ⋅ e2 => ⟦x:=v⟧ e1 ⋅ ⟦x:=v⟧ e2
+  | Bool b  => Bool b
+  | Nat n   => Nat n
+  | Cond e1 e2 e3 => Cond (⟦x:=v⟧ e1) (⟦x:=v⟧ e2) (⟦x:=v⟧ e3)
+  | Op o e1 e2    => Op o (⟦x:=v⟧ e1) (⟦x:=v⟧ e2)
+  | LET y e1 e2   => LET y (⟦x:=v⟧ e1) (if equiv_dec x y then e2 else ⟦x:=v⟧ e2)
+  end
+where "'⟦' x ':=' v '⟧' e" := (sub x v e).
+
+Open Scope maybe_scope.
+Open Scope op_scope.
+
+(** Call-by-name Evaluation. *)
+Fixpoint rd (e : term) : option term :=
+  match e with
+  | Var _ | λ _ ⇒ _ | Bool _ | Nat _ => None
+  | (λ x ⇒ e1) ⋅ e2 => Some (⟦x:=e2⟧ e1)
+  | e1 ⋅ e2 => let! e1' := rd e1 in e1' ⋅ e2
+  | Cond true  e2 _ => Some e2
+  | Cond false _ e3 => Some e3
+  | Cond e1 e2 e3 => let! e1' := rd e1 in Cond e1' e2 e3
+  | LET x e1 e2 => Some (⟦x:=e1⟧ e2)
+  | Op ⨥ (Nat n1)  (Nat n2)  => Some (Nat  (n1 + n2))
+  | Op ⨪ (Nat n1)  (Nat n2)  => Some (Nat  (n1 - n2))
+  | Op ∧ (Bool b1) (Bool b2) => Some (Bool (b1 &&  b2))
+  | Op ∨ (Bool b1) (Bool b2) => Some (Bool (b1 || b2))
+  | Op ≅ (Nat n1)  (Nat n2)  => Some (Bool (n1 =? n2))
+  | Op ≦ (Nat n1)  (Nat n2)  => Some (Bool (n1 <=? n2))
+  | Op o ((Nat _ | Bool _) as e1) e2 =>
+    let! e2' := rd e2 in Op o e1 e2'
+  | Op o e1 e2 => let! e1' := rd e1 in Op o e1' e2
+  end.
+
+Inductive value : term -> Prop :=
+| v_abs x e : value (λ x ⇒ e)
+| v_nat (n : nat) : value n
+| v_bool (b : bool) : value b.
